Implement automation, remove wp_gen

EvenOddProgram.thy
@@ -8,19 +8,19 @@ definition odd_entry :: "llvm_instruction_block" where
   "odd_entry \<equiv> (
     [],
     [
-      alloca (%''n.addr'') i32 (Some 4),
-      store i32 (reg %''n'') (reg %''n.addr'') (Some 4),
-      load (%''0'') i32 (reg %''n.addr'') (Some 4),
-      call (Some %''call'') i1 (@''even'') [(i32, reg %''0'')],
-      icmp (%''lnot'') False comp_eq i1 (reg %''call'') (val (vi1 False))
+      alloca (lid ''n.addr'') i32 (Some 4),
+      store i32 (reg (lid ''n'')) (reg (lid ''n.addr'')) (Some 4),
+      load (lid ''0'') i32 (reg (lid ''n.addr'')) (Some 4),
+      call (Some (lid ''call'')) i1 (gid ''even'') [(i32, reg (lid ''0''))],
+      icmp (lid ''lnot'') False comp_eq i1 (reg (lid ''call'')) (val (vi1 False))
     ],
-    ret (Some (i1, (reg %''lnot'')))
+    ret (Some (i1, (reg (lid ''lnot''))))
   )"
 
 definition odd_func :: "llvm_function" where
-  "odd_func \<equiv> func i1 [(%''n'', i32)]
+  "odd_func \<equiv> func i1 [(lid ''n'', i32)]
     [
-      (%''entry'', odd_entry)
+      (lid ''entry'', odd_entry)
     ]"
 
 
@@ -28,60 +28,196 @@ definition even_entry :: "llvm_instruction_block" where
   "even_entry \<equiv> (
     [],
     [
-      alloca (%''retval'') i1 (Some 1),
-      alloca (%''n.addr'') i32 (Some 4),
-      store i32 (reg %''n'') (reg %''n.addr'') (Some 4),
-      load (%''0'') i32 (reg %''n.addr'') (Some 4),
-      icmp (%''cmp'') False comp_eq i32 (reg %''0'') (val (vi32 0))
+      alloca (lid ''retval'') i1 (Some 1),
+      alloca (lid ''n.addr'') i32 (Some 4),
+      store i32 (reg (lid ''n'')) (reg (lid ''n.addr'')) (Some 4),
+      load (lid ''0'') i32 (reg (lid ''n.addr'')) (Some 4),
+      icmp (lid ''cmp'') False comp_eq i32 (reg (lid ''0'')) (val (vi32 0))
     ],
-    br_i1 (reg %''cmp'') (%''if.then'') (%''if.else'')
+    br_i1 (reg (lid ''cmp'')) (lid ''if.then'') (lid ''if.else'')
   )"
 definition even_if :: "llvm_instruction_block" where
   "even_if \<equiv> (
     [],
     [
-      store i1 (val (vi1 True)) (reg %''retval'') (Some 1)
+      store i1 (val (vi1 True)) (reg (lid ''retval'')) (Some 1)
     ],
-    br_label (%''return'')
+    br_label (lid ''return'')
   )"
 definition even_else :: "llvm_instruction_block" where
   "even_else \<equiv> (
     [],
     [
-      load (%1 ) i32 (reg %n.addr ) (Some 4),
-      add (%''sub'') add_nsw i32 (reg %''1'') (val (vi32 (-1))),
-      call (Some %''call'') i1 (@odd) [(i32, reg %''sub'')],
-      store i1 (reg %''call'') (reg %''retval'') (Some 1)
+      load (lid ''1'') i32 (reg (lid ''n.addr'')) (Some 4),
+      add (lid ''sub'') add_nsw i32 (reg (lid ''1'')) (val (vi32 (-1))),
+      call (Some (lid ''call'')) i1 (gid ''odd'') [(i32, reg (lid ''sub''))],
+      store i1 (reg (lid ''call'')) (reg (lid ''retval'')) (Some 1)
     ],
-    br_label ( %return )
+    br_label (lid ''return'')
   )"
 definition even_return :: "llvm_instruction_block" where
   "even_return \<equiv> (
     [],
     [
-      load (%''2'') i32 (reg %retval ) (Some 4)
+      load (lid ''2'') i32 (reg (lid ''retval'')) (Some 4)
     ],
-    ret (Some (i1, (reg %2)))
+    ret (Some (i1, (reg (lid ''2''))))
   )"
 
 definition even_func :: "llvm_function" where
-  "even_func \<equiv> func i1 [(%''n'', i32)]
+  "even_func \<equiv> func i1 [(lid ''n'', i32)]
     [
-      (%''entry'', even_entry),
-      (%''if.then'', even_if),
-      (%''if.else'', even_else),
-      (%''return'', even_return)
+      (lid ''entry'', even_entry),
+      (lid ''if.then'', even_if),
+      (lid ''if.else'', even_else),
+      (lid ''return'', even_return)
     ]"
 
 abbreviation even_annots :: "precondition * block_preconditions * postcondition" where
   "even_annots \<equiv> (
     (\<lambda>s.
-      \<exists>n. register_\<alpha> s (reg %''n'') = Some (vi32 n)
+      \<exists>n. register_\<alpha> s (reg (lid ''n'')) = Some (vi32 n)
     \<and> 0 \<le>s n
     ),
     [],
     (\<lambda>s s' v.
-      \<exists>n b a1 a2. register_\<alpha> s (reg %''n'') = Some (vi32 n)
+      \<exists>n b a1 a2. register_\<alpha> s (reg (lid ''n'')) = Some (vi32 n)
+    \<and> v = Some (vi1 (even n))
+    \<and> memory_\<alpha> s' = (memory_\<alpha> s)(saddr a1 := Some (mem_val (vi32 n)), saddr a2 := Some (mem_val (vi1 b)))
+    \<and> memory_\<alpha> s (saddr a1) = None
+    \<and> memory_\<alpha> s (saddr a2) = None
+    \<and> (\<forall>n. register_\<alpha> s' (reg (gid n)) = register_\<alpha> s (reg (gid n)))
+    )
+  )"
+abbreviation odd_annots :: "precondition * block_preconditions * postcondition" where
+  "odd_annots \<equiv> (
+    (\<lambda>s.
+      \<exists>n. register_\<alpha> s (reg (lid ''n'')) = Some (vi32 n)
+    \<and> 0 \<le>s n
+    ),
+    [],
+    (\<lambda>s s' v.
+      \<exists>n ad. register_\<alpha> s (reg (lid ''n'')) = Some (vi32 n)
+    \<and> v = Some (vi1 (odd n))
+    \<and> memory_\<alpha> s' = (memory_\<alpha> s)(saddr ad := Some (mem_val (vi32 n)))
+    \<and> memory_\<alpha> s (saddr ad) = None
+    \<and> (\<forall>n. register_\<alpha> s' (reg (gid n)) = register_\<alpha> s (reg (gid n)))
+    )
+  )"
+
+definition even_odd_prog :: "llvm_program" where
+  "even_odd_prog \<equiv> [
+    (gid ''even'', even_func),
+    (gid ''odd'',  odd_func)
+  ]"
+
+definition even_odd_annots :: "annotations" where
+  "even_odd_annots \<equiv> [
+    (gid ''even'', even_annots),
+    (gid ''odd'',  odd_annots)
+  ]"
+
+
+
+
+
+
+
+lemma verify_even_odd:
+  "verify_program even_odd_prog even_odd_annots"
+  apply (vcg_verify_program prog: even_odd_prog_def)
+
+  subgoal (* even function *)
+    apply (vcg_verify_function blocks: even_entry_def even_if_def even_else_def even_return_def prog: even_odd_prog_def annot: even_odd_annots_def func: even_func_def odd_func_def)
+    apply (auto split: if_splits simp: even_odd_prog_def)
+    apply (smt (verit, del_insts) add.inverse_neutral add_diff_cancel_right' diff_minus_eq_add fun_upd_same signed.nle_le signed_arith_eq_checks_to_ord(1) signed_minus_1
+          word_sle_eq)
+    by (simp add: word_sless_alt word_sle_eq signed.leD)
+  subgoal (* odd function *)
+    apply (vcg_verify_function blocks: odd_entry_def prog: even_odd_prog_def annot: even_odd_annots_def func: even_func_def odd_func_def)
+    unfolding even_odd_prog_def
+    by (auto split: if_splits)
+
+  done
+
+
+(*
+define dso_local noundef zeroext i1 @odd(int)(i32 noundef lid n) {
+entry:
+  lid n.addr = alloca i32, align 4
+  store i32 lid n, ptr lid n.addr, align 4
+  lid 0 = load i32, ptr lid n.addr, align 4
+  lid sub = sub nsw i32 lid 0, 1
+  lid call = call noundef zeroext i1 @even(int)(i32 noundef lid sub)
+  lid lnot = xor i1 lid call, true
+  ret i1 lid lnot
+}
+
+define dso_local noundef zeroext i1 @even(int)(i32 noundef lid n) {
+entry:
+  lid retval = alloca i1, align 1
+  lid n.addr = alloca i32, align 4
+  store i32 lid n, ptr lid n.addr, align 4
+  lid 0 = load i32, ptr lid n.addr, align 4
+  lid cmp = icmp eq i32 lid 0, 0
+  br i1 lid cmp, label lid if.then, label lid if.else
+
+if.then:
+  store i1 true, ptr lid retval, align 1
+  br label lid return
+
+if.else:
+  lid 1 = load i32, ptr lid n.addr, align 4
+  lid call = call noundef zeroext i1 @odd(int)(i32 noundef lid 1)
+  lid lnot = xor i1 lid call, true
+  store i1 lid lnot, ptr lid retval, align 1
+  br label lid return
+
+return:
+  lid 2 = load i1, ptr lid retval, align 1
+  ret i1 lid 2
+}
+
+
+
+
+bool even(int n);
+
+/*@
+assumes n \<ge> 0;
+asserts \result = odd n;
+asserts \<exists>a1 n. \resmem = (\inimem)(stack a1 \<mapsto> int n);
+asserts \resglo = \iniglo
+*/
+bool odd(int n) {
+    return !even(n);
+}
+
+/*@
+assumes n \<ge> 0;
+asserts \result = even n;
+asserts \resmem = (\inimem)(stack a1 \<mapsto> int n, stack a2 \<mapsto> bool b);
+asserts \resglo = \iniglo
+*/
+bool even(int n) {
+    if (n == 0) {
+        return true;
+    } else {
+        return odd(n-1);
+    }
+}
+
+
+
+abbreviation even_annots :: "precondition * block_preconditions * postcondition" where
+  "even_annots \<equiv> (
+    (\<lambda>s.
+      \<exists>n. register_\<alpha> s (reg (lid ''n'')) = Some (vi32 n)
+    \<and> 0 \<le>s n
+    ),
+    [],
+    (\<lambda>s s' v.
+      \<exists>n b a1 a2. register_\<alpha> s (reg (lid ''n'')) = Some (vi32 n)
     \<and> v = Some (vi1 (even n))
     \<and> memory_\<alpha> s' = (memory_\<alpha> s)(saddr a1 := Some (mem_val (vi32 n)), saddr a2 := Some (mem_val (vi1 b)))
     \<and> memory_\<alpha> s (saddr a1) = None
@@ -92,280 +228,18 @@ abbreviation even_annots :: "precondition * block_preconditions * postcondition"
 abbreviation odd_annots :: "precondition * block_preconditions * postcondition" where
   "odd_annots \<equiv> (
     (\<lambda>s.
-      \<exists>n. register_\<alpha> s (reg %''n'') = Some (vi32 n)
+      \<exists>n. register_\<alpha> s (reg (lid ''n'')) = Some (vi32 n)
     \<and> 0 \<le>s n
     ),
     [],
     (\<lambda>s s' v.
-      \<exists>n ad. register_\<alpha> s (reg %''n'') = Some (vi32 n)
+      \<exists>n ad. register_\<alpha> s (reg (lid ''n'')) = Some (vi32 n)
     \<and> v = Some (vi1 (odd n))
     \<and> memory_\<alpha> s' = (memory_\<alpha> s)(saddr ad := Some (mem_val (vi32 n)))
     \<and> memory_\<alpha> s (saddr ad) = None
     \<and> (\<forall>n. register_\<alpha> s' (reg @n) = register_\<alpha> s (reg @n))
     )
   )"
-
-definition even_odd_prog :: "llvm_program" where
-  "even_odd_prog \<equiv> [
-    (@''even'', even_func),
-    (@''odd'',  odd_func)
-  ]"
-
-definition even_odd_annots :: "annotations" where
-  "even_odd_annots \<equiv> [
-    (@''even'', even_annots),
-    (@''odd'',  odd_annots)
-  ]"
-
-lemma register_\<alpha>_pop_contract [simp]:
-  "register_\<alpha> (pop_frame s s') ref = (
-     case ref of
-       reg (lid n) \<Rightarrow> register_\<alpha> s (reg (lid n))
-     | reg (gid n) \<Rightarrow> register_\<alpha> s' (reg (gid n))
-     | val v       \<Rightarrow> Some v)"
-  by (cases s; cases s'; cases ref; auto split: llvm_value_ref.splits llvm_identifier.splits) 
-fun stack_len :: "state \<Rightarrow> nat" where
-  "stack_len (lr, gr, sm, hm, gm) = length sm"
-
-lemma memory_\<alpha>_pop_saddr [simp]:
-  "memory_\<alpha> (pop_frame s s') (saddr a) = 
-     (if memory_\<alpha> s (saddr a) \<noteq> None then memory_\<alpha> s' (saddr a) else None)"
-  by (cases s; cases s'; simp add: single_memory_\<alpha>_def allocated_single_memory_address_def)
-
-lemma memory_\<alpha>_pop_haddr [simp]:
-  "memory_\<alpha> (pop_frame s s') (haddr a) = memory_\<alpha> s' (haddr a)"
-  by (cases s; cases s'; simp)
-
-lemma memory_\<alpha>_pop_gaddr [simp]:
-  "memory_\<alpha> (pop_frame s s') (gaddr a) = memory_\<alpha> s' (gaddr a)"
-  by (cases s; cases s'; simp)
-
-
-lemma register_\<alpha>_push_frame [simp]:
-  "register_\<alpha> (push_frame s) (reg (lid n)) = None"
-  "register_\<alpha> (push_frame s) (reg (gid n)) = register_\<alpha> s (reg (gid n))"
-  by (cases s; simp)+
-
-lemma memory_\<alpha>_push_frame [simp]:
-  "memory_\<alpha> (push_frame s) = memory_\<alpha> s"
-  apply (rule ext) subgoal for ad
-    by (cases s; cases ad; simp)
-  done
-
-
-
-
-
-lemma contract_updates_register[simp]:
-  assumes trace_link: "\<And>r. register_\<alpha> callee_state (reg @r) = f (reg @r)"
-  assumes frame_invariant: "\<And>r name. r = reg @name \<Longrightarrow> f r = register_\<alpha> caller_state r"
-  shows "register_\<alpha> (pop_frame caller_state callee_state) = register_\<alpha> caller_state"
-  apply (rule ext)
-  subgoal for n apply (cases n)
-  subgoal for name apply (cases name)
-    using assms by (auto )
-  by simp done
-
-lemma pop_frame_peel_gaddr [simp]:
-  "(\<lambda>a. case a of saddr sa \<Rightarrow> if M a \<noteq> None then (C (gaddr ga \<mapsto> v)) a else None | _ \<Rightarrow> (C (gaddr ga \<mapsto> v)) a) =
-   ((\<lambda>a. case a of saddr sa \<Rightarrow> if M a \<noteq> None then C a else None | _ \<Rightarrow> C a) (gaddr ga \<mapsto> v))"
-  apply (rule ext) subgoal for a by (cases a) auto done
-
-lemma pop_frame_peel_haddr [simp]:
-  "(\<lambda>a. case a of saddr sa \<Rightarrow> if M a \<noteq> None then (C (haddr ha \<mapsto> v)) a else None | _ \<Rightarrow> (C (haddr ha \<mapsto> v)) a) =
-   ((\<lambda>a. case a of saddr sa \<Rightarrow> if M a \<noteq> None then C a else None | _ \<Rightarrow> C a) (haddr ha \<mapsto> v))"
-  apply (rule ext) subgoal for a by (cases a) auto done
-
-lemma pop_frame_peel_saddr [simp]:
-  "(\<lambda>a. case a of saddr sa' \<Rightarrow> if M a \<noteq> None then (C (saddr sa \<mapsto> v)) a else None | _ \<Rightarrow> (C (saddr sa \<mapsto> v)) a) =
-   (if M (saddr sa) \<noteq> None 
-    then ((\<lambda>a. case a of saddr sa' \<Rightarrow> if M a \<noteq> None then C a else None | _ \<Rightarrow> C a) (saddr sa \<mapsto> v))
-    else (\<lambda>a. case a of saddr sa' \<Rightarrow> if M a \<noteq> None then C a else None | _ \<Rightarrow> C a))"
-  apply (rule ext) subgoal for a by (cases a) auto done
-
-lemma pop_frame_M_drop_saddr [simp]:
-  "C (saddr sa') = None \<Longrightarrow>
-   (\<lambda>a. case a of saddr sa \<Rightarrow> if (M(saddr sa' \<mapsto> v)) a \<noteq> None then C a else None | _ \<Rightarrow> C a) =
-   (\<lambda>a. case a of saddr sa \<Rightarrow> if M a \<noteq> None then C a else None | _ \<Rightarrow> C a)"
-  apply (rule ext) subgoal for a by (cases a) auto done
-
-lemma pop_frame_peel_absolute_base [simp]:
-  "(\<lambda>a. case a of saddr sa \<Rightarrow> if C a \<noteq> None then C a else None | _ \<Rightarrow> C a) = C"
-  apply (rule ext) subgoal for a by (cases a) auto done
-
-lemma memory_pop_frame [simp]:
-  assumes "memory_\<alpha> x = X"
-  assumes "memory_\<alpha> y = Y"
-  shows "memory_\<alpha> (pop_frame x y) = (\<lambda>a. case a of saddr sa \<Rightarrow> if X a \<noteq> None then Y a else None | _ \<Rightarrow> Y a)"
-  apply (rule ext) subgoal for a using assms by (cases a) auto done
-
-
-lemma verify_even_odd:
-  "verify_program even_odd_prog even_odd_annots"
-  apply (vcg_verify_program prog: even_odd_prog_def annot: even_odd_annots_def)
-  apply (unfold_first_label func: even_func_def)
-    apply (unfold_first_label func: even_func_def)
-    apply (intro allI impI)
-  subgoal for s
-    apply (vcg_floyd_cond prog: even_odd_prog_def func: even_func_def)
-    apply clean_assms
-    apply (vcg_steps_execi block: even_entry_def)
-    apply vcg_steps_execi
-    apply vcg_steps_execi
-    apply vcg_steps_execi
-    apply vcg_steps_execi
-    apply vcg_steps_execi
-    subgoal for n rva na s'
-      apply (vcg_steps_flowi_branch prog: even_odd_prog_def annot: even_odd_annots_def)
-      apply (vcg_step prog: even_odd_prog_def func: even_func_def)
-      apply (vcg_steps_execi block: even_if_def)
-      apply vcg_steps_execi
-      apply (vcg_steps_flowi_branch prog: even_odd_prog_def annot: even_odd_annots_def)
-      apply (vcg_step prog: even_odd_prog_def func: even_func_def)
-      apply (vcg_steps_execi block: even_return_def)
-      apply vcg_steps_execi
-      apply (vcg_steps_flowi_return prog: even_odd_prog_def annot: even_odd_annots_def)
-      apply (vcg_annotation_holds prog: even_odd_prog_def annot: even_odd_annots_def pre: even_odd_annots_def)
-      unfolding even_odd_prog_def
-      by (auto split: if_splits)
-    subgoal for n rva na s'
-      apply (vcg_steps_flowi_branch prog: even_odd_prog_def annot: even_odd_annots_def)
-      apply (vcg_step prog: even_odd_prog_def func: even_func_def)
-      apply (vcg_steps_execi block: even_else_def)
-      apply (vcg_steps_execi)
-      apply (vcg_steps_execi)
-         apply (subst even_odd_prog_def)
-         apply simp
-        apply (unfold_first_label func: odd_func_def)
-       apply (subst even_odd_annots_def)
-       apply simp
-      apply (simp only: prepare_state.simps)
-      apply (subst odd_func_def)
-      apply (simp (no_asm) del: assign_params.simps split_paired_All)
-      apply (intro wp_assign_params_intro wp_assign_params_empty_intro) apply simp apply simp
-      apply (intro conjI)
-      apply (smt (verit, del_insts) add.inverse_neutral add_diff_cancel_right' diff_minus_eq_add fun_upd_same signed.nle_le signed_arith_eq_checks_to_ord(1) signed_minus_1
-          word_sle_eq)
-      apply (intro allI impI)
-      apply (elim exE conjE)
-      apply (rule wp_restore_state_intro)
-        apply blast defer
-       apply blast
-      apply (intro wp_intro)
-        apply fastforce defer
-       apply blast
-        apply (elim conjE)
-  apply simp
-  apply (hypsubst_thin)+
-  apply (subst (asm) fun_upd_apply[symmetric])+
-  apply clean_assms
-      apply vcg_steps_execi
-      apply vcg_steps_execi
-      apply (vcg_steps_flowi_branch prog: even_odd_prog_def annot: even_odd_annots_def)
-      apply (vcg_step prog: even_odd_prog_def func: even_func_def)
-      apply (vcg_steps_execi block: even_return_def)
-
-      apply vcg_steps_execi
-      apply (vcg_steps_flowi_return prog: even_odd_prog_def annot: even_odd_annots_def)
-      apply (vcg_annotation_holds prog: even_odd_prog_def annot: even_odd_annots_def pre: even_odd_annots_def)
-      unfolding even_odd_prog_def apply (intro conjI) apply simp apply blast apply (auto split: if_splits)
-      by fast
-    done
-  apply (unfold_first_label func: odd_func_def)
-  apply (unfold_first_label func: odd_func_def)
-  apply (intro allI impI)
-  subgoal for s
-    apply (vcg_floyd_cond prog: even_odd_prog_def func: odd_func_def)
-    apply clean_assms
-    apply (vcg_steps_execi block: odd_entry_def)
-    apply vcg_steps_execi
-    apply vcg_steps_execi
-    apply vcg_steps_execi
-         apply (subst even_odd_prog_def)
-         apply simp
-        apply (unfold_first_label func: even_func_def)
-       apply (subst even_odd_annots_def)
-       apply simp
-      apply (simp only: prepare_state.simps)
-      apply (subst even_func_def)
-      apply (simp (no_asm) del: assign_params.simps split_paired_All)
-      apply (intro wp_assign_params_intro wp_assign_params_empty_intro) apply simp apply simp
-    apply (intro conjI)
-     apply simp
-      apply (intro allI impI)
-      apply (elim exE conjE)
-      apply (rule wp_restore_state_intro)
-        apply blast defer
-       apply blast
-      apply (intro wp_intro)
-        apply fastforce defer
-       apply blast
-        apply (elim conjE)
-  apply simp
-  apply (hypsubst_thin)+
-  apply (subst (asm) fun_upd_apply[symmetric])+
-  apply clean_assms
-  apply vcg_steps_execi
-  apply vcg_steps_execi
-      apply (vcg_steps_flowi_return prog: even_odd_prog_def annot: even_odd_annots_def)
-      apply (vcg_annotation_holds prog: even_odd_prog_def annot: even_odd_annots_def pre: even_odd_annots_def)
-      unfolding even_odd_prog_def by (auto split: if_splits)
-    done  
-
-
-(*
-define dso_local noundef zeroext i1 @odd(int)(i32 noundef %n) {
-entry:
-  %n.addr = alloca i32, align 4
-  store i32 %n, ptr %n.addr, align 4
-  %0 = load i32, ptr %n.addr, align 4
-  %sub = sub nsw i32 %0, 1
-  %call = call noundef zeroext i1 @even(int)(i32 noundef %sub)
-  %lnot = xor i1 %call, true
-  ret i1 %lnot
-}
-
-define dso_local noundef zeroext i1 @even(int)(i32 noundef %n) {
-entry:
-  %retval = alloca i1, align 1
-  %n.addr = alloca i32, align 4
-  store i32 %n, ptr %n.addr, align 4
-  %0 = load i32, ptr %n.addr, align 4
-  %cmp = icmp eq i32 %0, 0
-  br i1 %cmp, label %if.then, label %if.else
-
-if.then:
-  store i1 true, ptr %retval, align 1
-  br label %return
-
-if.else:
-  %1 = load i32, ptr %n.addr, align 4
-  %call = call noundef zeroext i1 @odd(int)(i32 noundef %1)
-  %lnot = xor i1 %call, true
-  store i1 %lnot, ptr %retval, align 1
-  br label %return
-
-return:
-  %2 = load i1, ptr %retval, align 1
-  ret i1 %2
-}
-
-
-
-
-bool even(int n);
-
-bool odd(int n) {
-    return !even(n);
-}
-
-bool even(int n) {
-    if (n == 0) {
-        return true;
-    } else {
-        return odd(n-1);
-    }
-}
 
 *)
 
